Add `Attribute` and `TypeAttr` inductive types
These two types are used to represent attributes and types in the IR,
respectively. This is not the final design, as they should be extensible
and not require to recompile the whole codebase whenever a new attribute
or type is added. However, this is a first step to at least be able to
represent attributes and types in the IR.

Similar to xDSl, I merged Attribute and Type into a single type, so that
we can write functions that can both operate on attributes and types
without having to duplicate code.

Veir/Rewriter/Basic.lean
@@ -380,7 +380,7 @@ theorem Rewriter.initOpRegions_inBounds_mono (ptr : GenericPtr) :
     ptr.InBounds ctx → ptr.InBounds (initOpRegions ctx opPtr regions n opPtrInBounds hregions hctx hn) := by
   induction n generalizing ctx <;> simp only [initOpRegions] <;> grind
 
-def Rewriter.initOpResults (ctx: IRContext) (opPtr: OperationPtr) (resultTypes: Array MlirType) (index: Nat := 0) (hop : opPtr.InBounds ctx)
+def Rewriter.initOpResults (ctx: IRContext) (opPtr: OperationPtr) (resultTypes: Array TypeAttr) (index: Nat := 0) (hop : opPtr.InBounds ctx)
     (hidx : index = opPtr.getNumResults ctx) : IRContext :=
   if h: index >= resultTypes.size then
     ctx
@@ -559,7 +559,7 @@ theorem Rewriter.createEmptyOp_fieldsInBounds (h : createEmptyOp ctx opType = so
 
 @[irreducible]
 def Rewriter.createOp (ctx: IRContext) (opType: OpCode)
-    (resultTypes: Array MlirType) (operands: Array ValuePtr) (blockOperands : Array BlockPtr)
+    (resultTypes: Array TypeAttr) (operands: Array ValuePtr) (blockOperands : Array BlockPtr)
     (regions: Array RegionPtr) (properties: UInt64)
     (insertionPoint: Option InsertPoint)
     (hoper : ∀ oper, oper ∈ operands → oper.InBounds ctx)
