Veir/IR/Attribute.lean
@@ -1,0 +1,90 @@
+module
+
+/-!
+  # Attributes
+
+  This file defines the `Attribute` data structure, which is an inductive type
+  that can represent any compile-time information that can be stored in the IR.
+  Attributes are used either as type annotations for SSA values, or as extra
+  information stored in operations.
+
+  The `TypeAttr` definition is a subtype of `Attribute` that carries the additional
+  invariant that the attribute is a valid type annotation.
+
+  `TypeAttr` corresponds to `mlir::Type`, and `Attribute`s that are not
+  `TypeAttr`s correspond to an `mlir::Attribute` (as attributes and types are
+  completely disjoint in MLIR). The reason for this lack of separation in VeIR is
+  that merging both concepts into a single `Attribute` type allows to define
+  functions that can work with both types and attributes without needing to define
+  separate functions for each case.
+-/
+
+namespace Veir
+public section
+
+/--
+  A data structure that represents compile-time information in the IR.
+  Attributes are used either as type annotations for SSA values, or
+  as extra information stored in operations.
+-/
+inductive Attribute
+| integerType (bitwidth : Nat)
+/--
+  An attribute from an unknown dialect.
+-/
+| unregistered (value : String) (isType : Bool)
+deriving Inhabited, Repr, DecidableEq, Hashable
+
+namespace Attribute
+
+/--
+  Determine if an attribute can be used as a type annotation for SSA
+  values.
+-/
+def isType (attr : Attribute) : Bool :=
+  match attr with
+  | .integerType _ => true
+  | .unregistered _ isType => isType
+
+@[simp, grind =]
+theorem isType_integerType bitwidth : (integerType bitwidth).isType = true := by rfl
+@[simp, grind =]
+theorem isType_unregistered value isType : (unregistered value isType).isType = isType := by rfl
+
+/--
+  Convert an attribute to a string representation.
+-/
+def toString (attr : Attribute) : String :=
+  match attr with
+  | .integerType bitwidth => s!"i{bitwidth}"
+  | .unregistered value _ => value
+
+instance : ToString Attribute where
+  toString := toString
+
+end Attribute
+
+/--
+  An attribute that can be used as a type annotation for SSA values.
+-/
+@[expose]
+def TypeAttr := {attr // Attribute.isType attr}
+deriving Repr, Hashable, DecidableEq
+
+instance : Inhabited TypeAttr where
+  default := ⟨.integerType 0, by rfl⟩
+
+instance : Coe TypeAttr Attribute where
+  coe typeAttr := typeAttr.val
+
+instance : ToString TypeAttr where
+  toString typeAttr := toString (typeAttr.val)
+
+/--
+  Convert an attribute to a type attribute.
+-/
+def Attribute.asType (attr : Attribute) (isType : attr.isType := by grind) : TypeAttr :=
+  ⟨attr, isType⟩
+
+end
+end Veir
