Veir/PatternRewriter/Basic.lean
@@ -142,7 +142,7 @@ theorem addUsersInWorklist_same_ctx :
   simp [addUsersInWorklist]
 
 def createOp (rewriter: PatternRewriter) (opType: OpCode)
-    (resultTypes: Array MlirType) (operands: Array ValuePtr) (blockOperands: Array BlockPtr) (regions: Array RegionPtr) (properties: UInt64)
+    (resultTypes: Array TypeAttr) (operands: Array ValuePtr) (blockOperands: Array BlockPtr) (regions: Array RegionPtr) (properties: UInt64)
     (insertionPoint: Option InsertPoint)
     (hoper : ∀ oper, oper ∈ operands → oper.InBounds rewriter.ctx)
     (hblockOperands : ∀ blockOper, blockOper ∈ blockOperands → blockOper.InBounds rewriter.ctx)
