Veir/Rewriter/WellFormed/Builder/Operation.lean
@@ -12,7 +12,7 @@ theorem OperationPtr.setProperties_WellFormed (op: OperationPtr) (ctx: IRContext
 
 set_option warn.sorry false in
 theorem Rewriter.createOp_WellFormed (ctx: IRContext) (opType: OpCode)
-    (resultTypes: Array MlirType) (operands: Array ValuePtr) (numRegions: Nat) (properties: UInt64)
+    (resultTypes: Array TypeAttr) (operands: Array ValuePtr) (numRegions: Nat) (properties: UInt64)
     (insertionPoint: Option InsertPoint)
     (hoper : ∀ oper, oper ∈ operands → oper.InBounds ctx)
     hblockOper
